# AERE 310 HW 1

Abhigyaan Deep

## 1.

Given:

$$
f(x,y) = xy
$$

## 1. (a)

$$
f(x,y) = c = xy
$$

$$
y = \frac{c}{x}
$$

I chose all integers in $[-3, 3]$ to generate [the following Desmos level surfaces](https://www.desmos.com/calculator/yg04m60tc2):

![Level Surfaces](https://i.imgur.com/LiMsHTxl.png)

## 1. (b)

$$
\nabla f(x,y) = \langle \frac{\partial}{\partial x} xy, \frac{\partial}{\partial y} xy \rangle = \langle y, x \rangle
$$

[A GeoGebra applet](https://www.geogebra.org/m/QPE4PaDZ) conveys the gradient well:

![Gradient Vectors](https://i.imgur.com/VaIyaGbl.png)

## 2.

Given:

$$
\vec{V} = u \hat{i} = V_0 (1 - e^{-ct}) (1 - \frac{x}{l}) \hat{i}
$$

![Diffuser](https://i.imgur.com/RdS7XTRm.png)

## 2. (a)

We have already been given the velocity as a function of $x$ and $t$:

$$
\vec{V}(x,t) = V_0 (1 - e^{-ct}) (1 - \frac{x}{l}) \hat{i}
$$

Therefore, the acceleration can be derived directly:

$$
\vec{A}(x,t) = \frac{\partial \vec{V}}{\partial t}
$$

$$
\vec{A}(x,t) = V_0 \hat{i} \left[ \frac{\partial}{\partial t} \left((1-e^{-ct}) (1-\frac{x}{l}) \right) \right]
$$

$$
\vec{A}(x,t) = V_0 \hat{i} \left[ c e^{-ct} (1-\frac{x}{l}) + 0 \right]
$$

$$
\vec{A}(x,t) = \boxed{c V_0 e^{-ct} (1 - \frac{x}{l}) \hat{i}}
$$

# 2. (b)

$$
V_0=10ft/s
$$

$$
l=5ft
$$

$$
l=1s
$$

$$
c=0.49s^{-1}
$$

Here, $x=l$ since we are trying to find the "end" behavior by the end of the diffuser.

$$
\vec{A} = 0.49s^{-1} \times 10ft/s \times e^{-0.49s^{-1} \times 1s} (1 - \frac{5ft}{5ft}) \hat{i} = 0
$$

The $0$ originates from the fact that $x=l$. Thus, we end up dividing $l/l=1$. The equation then subtracts $1$ from $1$ to get $0$. Regardless of the values of other members of the product, the function returns $0$.

Intuitively, this behavior shouldn't be too otherworldly. An acceleration of $0$ does not imply a velocity of $0$. Sure, the liquid has stopped moving faster/slower, but it's still moving regardless. In other words, the diffuser has indeed diffused the liquid. Also the liquid is now starting to accelerate purely in the $\hat{j}$ direction.

## 3.

Given:

$$
u = \frac{cx}{x^2+y^2}
$$

$$
v = \frac{cy}{x^2+y^2}
$$

## 3. (a)

$$
V = \langle u, v \rangle
$$

$$
\frac{\Delta \delta V}{\Delta t} = \nabla \cdot V = \frac{\partial}{\partial x} \frac{cx}{x^2+y^2} + \frac{\partial}{\partial y} \frac{cy}{x^2+y^2}
$$

$$
\frac{\Delta \delta V}{\Delta t} = \frac{c (y^2 - x^2)}{(x^2 + y^2)^2} + \frac{c (x^2 - y^2)}{(x^2 + y^2)^2} = \frac{c (y^2 - x^2) + c (x^2 - y^2)}{(x^2 + y^2)^2} = \frac{c (y^2 - x^2 + x^2 - y^2)}{(x^2 + y^2)^2} = \boxed{0}
$$

$0$ makes sense as this is incompressible flow after all.

## 3. (b)

$$
w = \nabla \times V = \frac{\partial}{\partial x} v - \frac{\partial}{\partial y} u
$$

$$
w = \frac{\partial}{\partial x} \frac{cy}{x^2+y^2} - \frac{\partial}{\partial y} \frac{cx}{x^2+y^2}
$$

$$
w = \frac{-2cxy}{(x^2 + y^2)^2} - \frac{-2cxy}{(x^2 + y^2)^2} = \boxed{0}
$$

Once again, $0$ makes intuitive sense as the diffusor doesn't seem to have any geometry that could cause the liquid to "turn on itself" and moving retrograde to all other fluid particles.

## 4.

Given:

$$
d_p=55ft=16.76m
$$

$$
D_p=950lbf=4226N
$$

$$
u_p=12mi/h=5.364m/s
$$

$$
T_p=20\degree C=293.2K
$$

$$
p_p=1atm=101325Pa
$$

$$
d_m=1.7m
$$

$$
\rho=1kg/m^3
$$

$$
\mu=2*10^{-5}Pa*s
$$

## 4. (a)

$$
Re_m=Re_p
$$

$$
\frac{\rho u_m d_m}{\mu} = \frac{\rho u_p d_p}{\mu}
$$

$$
u_m = \frac{\cancel{\rho} u_p d_p \cancel{\mu}}{\cancel{\mu} \cancel{\rho} d_m} = \frac{u_p d_p}{d_m} = \frac{5.364m/s * 16.76m}{1.7m} = \boxed{52.9m/s}
$$

## 4. (b)

$$
D = \frac{1}{2} \rho u^2 C_D A
$$

$$
C_D = \frac{2D}{\rho u^2 A} = \frac{2D_p}{\rho u_p^2 \frac{\pi}{4} d_p^2} = \frac{2 * 4226N}{1kg/m^3 * (5.364m/s)^2 \frac{\pi}{4} * (16.76m)^2} = 1.3315
$$

$$
D_m = \frac{1}{2} \rho u_m^2 C_D \frac{\pi}{4} d_m^2 = \frac{1}{2} * 1kg/m^3 * (52.9m/s)^2 * 1.3315 * \frac{\pi}{4} (1.7m)^2 = \boxed{4230N}
$$

## 4. (c)

$D_m$ is suspiciously close to $D_p$ and I suspect this is due to some secret cancellations within the many fractions.

## 5.

$$
F[N] \implies MLT^{-2}
$$

$$
D[m] \implies L
$$

$$
\Omega[rad/s] \implies T^{-1}
$$

$$
V[m/s] \implies LT^{-1}
$$

$$
\rho[kg/m^3] \implies ML^{-3}
$$

$$
\mu[Pa*s] \implies ML^{-1}T^{-1}
$$

$F$ is dependant ($1$ variables). $D$, $\Omega$, $V$, $\rho$, and $\mu$ are independent ($5$ variables). This makes a total of $N=6$ variables. $M$, $L$, and $T$ are the fundamental dimensions ($k=3$ dimensions). Hence, there are $N-k=6-3=3$ dimensionless groups.

I am making the function $g$ use $F$ as an input; it should be solvable for it implemented. Also, I am using $g$ and $G$ for function names because $f$ and $F$ would be confusing as we're already using $F$ for force.

$$
g(F, D, \Omega, V, \rho, \mu) \implies G(\Pi_1, \Pi_2, \Pi_3)
$$

After much research, I settled on $D$, $V$, and $\rho$ for my repeating variables:

$$
\Pi_1 = g_1(D, V, \rho, F)
$$

$$
\Pi_2 = g_1(D, V, \rho, \Omega)
$$

$$
\Pi_3 = g_1(D, V, \rho, \mu)
$$

The question inquires about $F$ so I am going to only mess around with $\Pi_1$:

$$
\Pi_1 = D ~ V^a ~ \rho^b ~ F^c
$$

$$
[\Pi_1] = [D] ~ [V]^a ~ [\rho]^b ~ [F]^c
$$

$$
1 = L ~ (LT^{-1})^a ~ (ML^{-3})^b ~ (MLT^{-2})^c
$$

$$
1 = L L^a T^{-a} M^b L^{-3b} M^c L^c T^{-2c}
$$

$$
1 = L^{1 + a - 3b + c} T^{-a - 2c} M^{b + c}
$$

$$
1 + a - 3b + c = 0
$$

$$
-a - 2c = 0
$$

$$
b + c = 0
$$

$$
1 + a - 3b + c - a - 2c = 0
$$

$$
1 - 3b - c = 0
$$

$$
1 - 3b - c + b + c = 0
$$

$$
1 - 2b = 0
$$

$$
1 = 2b
$$

$$
b = \frac{1}{2}
$$

$$
\frac{1}{2} + c = 0
$$

$$
c = -\frac{1}{2}
$$

$$
-a - 2 * -\frac{1}{2} = 0
$$

$$
-a + 1 = 0
$$

$$
a = 1
$$

$$
\Pi_1 = D V \rho^{1/2} F^{-1/2} = \boxed{D V \sqrt{\frac{\rho}{F}}}
$$

Plugging in all base SI units does indeed give you $1$:

$$
1m * 1m/s * \sqrt{\frac{1kg/m^3}{1N}} = 1
$$
