# AERE 310 HW 3

Abhigyaan Deep

## 1.

$$
u=6xy
$$

$$
v=2x-3y^2
$$

## 1. (a)

$$
\frac{\partial u}{\partial x} + \frac{\partial v}{\partial y} = 0
$$

$$
\boxed{\cancel{6y} + \cancel{(-6y)} = 0}
$$

$$
u = \frac{\partial \psi}{\partial y}
$$

$$
\partial \psi = u \partial y = 6xy \partial y
$$

$$
\psi = 3xy^2 + f(x)
$$

$$
v = -\frac{\partial \psi}{\partial x} = -\frac{\partial (3xy^2 + f(x))}{\partial x}
$$

$$
v = \cancel{-3y^2} - f'(x) = 2x - \cancel{3y^3}
$$

$$
f'(x) = -2x
$$

$$
f(x) = -x^2 + c
$$

$$
\boxed{\psi = 3xy^2 - x^2 + c}
$$

## 1. (b)

The following Desmos stream lines use $c=0$ and $\Phi = \{ x \in \mathbb{Z} \mid -5 \leq x \leq 5 \}$ (all integers from $-5$ to $5$):

![](https://i.imgur.com/hXr9Gz8l.png)

https://www.desmos.com/calculator/zh0tdclq5f

## 2.

$$
v_r = 2r + 3r^2 \sin \theta
$$

$$
\frac{1}{r} \frac{\partial (r v_r)}{\partial r} + \frac{1}{r} \frac{\partial v_\theta}{\partial \theta} = 0
$$

$$
\frac{1}{r} \frac{\partial (r (2r + 3r^2 \sin \theta))}{\partial r} + \frac{1}{r} \frac{\partial v_\theta}{\partial \theta} = 0
$$

$$
\frac{1}{r} \frac{\partial (2r^2 + 3r^3 \sin \theta)}{\partial r} + \frac{1}{r} \frac{\partial v_\theta}{\partial \theta} = 0
$$

$$
\frac{1}{r} (4r + 9r^2 \sin \theta) + \frac{1}{r} \frac{\partial v_\theta}{\partial \theta} = 0
$$

$$
4 + 9r \sin \theta + \frac{1}{r} \frac{\partial v_\theta}{\partial \theta} = 0
$$

$$
\frac{1}{r} \frac{\partial v_\theta}{\partial \theta} = - =4 - 9r \sin \theta
$$

$$
\frac{\partial v_\theta}{\partial \theta} = -4r - 9r^2 \sin \theta
$$

$$
\partial v_\theta = (-4r - 9r^2 \sin \theta) \partial \theta
$$

$$
v_\theta = -4r\theta + 9r^2 \sin \theta + f(r)
$$

$$
\boxed{v_\theta = 9r^2 \sin \theta - 4r\theta + f(r)}
$$

## 3.

$$
u = x^2 - y^2 + x
$$

$$
v = -(2xy + y) = -2xy - y
$$

## 3. (a)

$$
\omega = \frac{\partial v}{\partial x} - \frac{\partial u}{\partial y} = 0
$$

$$
\frac{\partial (-2xy - y)}{\partial x} - \frac{\partial (x^2 - y^2 + x)}{\partial y} = 0
$$

$$
\boxed{\cancel{-2y} - \cancel{(-2y)} = 0}
$$

$$
u = \frac{\partial \phi}{\partial x}
$$

$$
\partial \phi = u \partial x = (x^2 - y^2 + x) \partial x
$$

$$
\phi = \frac{1}{3}x^3 - xy^2 + \frac{1}{2}x^2 + f(y)
$$

$$
v = \frac{\partial \phi}{\partial y} = \frac{\partial (\frac{1}{3}x^3 - xy^2 + \frac{1}{2}x^2 + f(y))}{\partial y}
$$

$$
v = \cancel{-2xy} + f'(y) = \cancel{-2xy} - y
$$

$$
f'(y) = -y
$$

$$
f(y) = -\frac{1}{2} y^2 + c
$$

$$
\boxed{\phi = \frac{1}{3}x^3 - xy^2 + \frac{1}{2}x^2 - \frac{1}{2} y^2 + c}
$$

## 3. (b)

$$
P_0 = (0, 0)
$$

$$
P_1 = (2, 3)
$$

$$
t_0 = 0
$$

$$
t_1 = 1
$$

$$
x(t) = 2t
$$

$$
dx(t) = 2
$$

$$
y(t) = 3t
$$

$$
dy(t) = 3
$$

$$
d\vec{s} = \langle 2, 3 \rangle dt
$$

$$
V = \langle u, v \rangle = \langle x^2 - y^2 + x, -2xy - y \rangle
$$

$$
V(t) = \langle (2t)^2 - (3t)^2 + 2t, -2(2t)(3t) - 3t \rangle
$$

$$
V(t) = \langle 4t^2 - 9t^2 + 2t, -12t^2 - 3t \rangle
$$

$$
V(t) = \langle -5t^2 + 2t, -12t^2 - 3t \rangle
$$

$$
I = \int_{(0, 0)}^{(2, 3)} V \cdot d\vec{s} = \int_0^1 V(t) \cdot \langle 2, 3 \rangle dt
$$

$$
I = \int_0^1 2(-5t^2 + 2t) + 3(-12t^2 - 3t) ~ dt
$$

$$
I = \int_0^1 -10t^2 + 4t + -36t^2 - 9t ~ dt
$$

$$
I = \int_0^1 -46t^2 - 5t ~ dt
$$

$$
I = \left[ -\frac{46}{3}t^3 - \frac{5}{2}t^2 \right]_0^1 = -\frac{46}{3} - \frac{5}{2}
$$

$$
\boxed{I = -\frac{107}{6}}
$$

## 3. (c)

$$
I_{I} = \int_{(0, 0)}^{(2, 0)} V \cdot d\vec{s} = \int_{x_0 = 0}^{x_1 = 2} (u + v) dx \quad \text{where y = 0}
$$

$$
I_{I} = \int_0^2 x^2 - 0^2 + x - 2x \cdot 0 - 0 ~ dx
$$

$$
I_{I} = \int_0^2 x^2 + x ~ dx
$$

$$
I_{I} = \left[ \frac{1}{3} x^3 + \frac{1}{2} x^2 \right]_0^2 = \frac{8}{3} + \frac{4}{2}
$$

$$
\boxed{I_{I} = \frac{14}{3}}
$$

$$
I_{II} = \int_{(2, 0)}^{(2, 3)} V \cdot d\vec{s} = \int_{y_0 = 0}^{y_1 = 3} (u + v) dy \quad \text{where x = 2}
$$

$$
I_{II} = \int_{0}^{3} 4 - y^2 + 2 - 4y - y ~ dy = \int_{0}^{3} 6 - y^2 - 5y ~ dy
$$

$$
I_{II} = \left[ 6y - \frac{1}{3}y^3 - \frac{5}{2}y^2 \right]_0^3
$$

$$
\boxed{I_{II} = -\frac{45}{2}}
$$

$$
\boxed{I_{I} + I_{II} = \frac{14}{3} - \frac{45}{2} = -\frac{107}{6} = I}
$$

This isn't surprisingly because $V$ is a conservative field which we studied extensively in Calc III; these vector felids don't care about your path of travel, the ends justify the means.

## 4.

$$
u(y) = U_m \left( 1 - \left( \frac{y}{H} \right)^2 \right) = U_m - \frac{U_m}{H^2}y^2
$$

$$
v=0
$$

## 4. (a)

$$
\Gamma = \oint_C V \cdot ds
$$

$$
\Gamma_A = \int_\text{bottom} u(-a/2) \hat{i} \cdot \hat{i} ~ dx + \int_\text{right} u(y) \cancel{\hat{i} \cdot \hat{j}} ~ dy + \int_\text{top} u(a/2) \hat{i} \cdot -\hat{i} ~ dx + \int_\text{left} u(y) \cancel{\hat{i} \cdot -\hat{j}} ~ dy
$$

$$
\Gamma_A = \int_0^a u(-a/2) dx - \int_0^a u(a/2) dx
$$

$$
\Gamma_A = \int_0^a U_m - \frac{U_m}{H^2}(-a/2)^2 dx - \int_0^a U_m - \frac{U_m}{H^2}(a/2)^2 dx
$$

$$
\Gamma_A = \cancel{\int_0^a U_m - \frac{U_m a^2}{4 H^2} dx} - \cancel{\int_0^a U_m - \frac{U_m a^2}{4 H^2} dx}
$$

$$
\boxed{\Gamma_A = 0}
$$

$$
\Gamma_B = \int_\text{bottom} u(0) \hat{i} \cdot \hat{i} ~ dx + \int_\text{right} u(y) \cancel{\hat{i} \cdot \hat{j}} ~ dy + \int_\text{top} u(a) \hat{i} \cdot -\hat{i} ~ dx + \int_\text{left} u(y) \cancel{\hat{i} \cdot -\hat{j}} ~ dy
$$

$$
\Gamma_B = \int_0^a u(0) dx - \int_0^a u(a) dx
$$

$$
\Gamma_B = u(0) \int_0^a dx - u(a) \int_0^a dx
$$

$$
\Gamma_B = u(0) a - u(a) a
$$

$$
\Gamma_B = a U_m - \cancel{\frac{a U_m}{H^2} \cdot 0^2} - (a U_m - \frac{a U_m}{H^2}a^2)
$$

$$
\Gamma_B = \cancel{a U_m} - \cancel{a U_m} + \frac{a U_m}{H^2}a^2
$$

$$
\boxed{\Gamma_B = -\frac{a^3 U_m}{H^2}}
$$

## 4. (b)

$$
\frac{\partial v}{\partial x} = 0
$$

$$
\frac{\partial u}{\partial y} = \frac{2 U_m}{H^2}y
$$

$$
\omega = \omega_z \hat{k} = \left( \frac{\partial v}{\partial x} - \frac{\partial u}{\partial y} \right) \hat{k} = -\frac{2 U_m}{H^2}y \hat{k}
$$

$$
\Gamma = \iint_S \omega \cdot \hat{n} dS
$$

$$
\Gamma_A = \int_0^a \int_{-a/2}^{a/2} -\frac{2 U_m}{H^2}y \hat{k} \cdot \hat{k} ~ dy ~ dx
$$

$$
\Gamma_A = \int_0^a \int_{-a/2}^{a/2} -\frac{2 U_m}{H^2}y ~ dy ~ dx
$$

$$
\Gamma_A = \int_0^a \left[ -\frac{U_m}{H^2}y^2 \right]_{-a/2}^{a/2} dx
$$

$$
\Gamma_A = \int_0^a \left[ \cancel{-\frac{U_m a^2}{4H^2}y^2} + \cancel{\frac{U_m a^2}{4H^2}y^2} \right] dx
$$

$$
\boxed{\Gamma_A = 0}
$$

$$
\Gamma_B = \int_0^a \int_0^a -\frac{2 U_m}{H^2}y \hat{k} \cdot \hat{k} ~ dy ~ dx
$$

$$
\Gamma_B = \int_0^a \int_0^a -\frac{2 U_m}{H^2}y ~ dy ~ dx
$$

$$
\Gamma_B = \int_0^a \left[ -\frac{U_m}{H^2}y^2 \right]_0^a dx
$$

$$
\Gamma_B = -\frac{a^2 U_m}{H^2} \int_0^a dx
$$

$$
\boxed{\Gamma_B = -\frac{a^3 U_m}{H^2}}
$$

It shouldn't be surprising that $\Gamma$ values across both parts of the question match since they both literally equal each other in the integral form. It also makes sense that $\Gamma_A = 0$ since it's symmetrical so there's no "spinny bits." Lastly, it makes sense that $\Gamma_B \neq 0$ since there's "shear" in the flow.

$$
\Gamma = \oint_C V \cdot ds = \iint_S \omega \cdot \hat{n} dS
$$

## 5.

$$
\psi(x, y) = 2xy^2 - \frac{2}{3}x^3
$$

$$
[x] = [y] = m
$$

$$
[\psi] = m^2/s
$$

$$
P_0 = (1, 1)
$$

$$
p_0 = 200kPa
$$

$$
P_1 = (2, 2)
$$

$$
\rho = 1000kg/m^3
$$

$$
u = \frac{\partial \psi}{\partial y} = 4xy
$$

$$
v = -\frac{\partial \psi}{\partial x} = -(2y^2 - 2x^2) = 2x^2 - 2y^2
$$

$$
V = \langle u, v \rangle = \langle 4xy, 2x^2 - 2y^2 \rangle
$$

$$
V_0 = V(P_0) = \langle 4, 2 - 2 \rangle = \langle 4, 0 \rangle \implies |V_0| = 4m/s
$$

$$
V_1 = V(P_1) = \langle 16, 8 - 8 \rangle = \langle 16, 0 \rangle \implies |V_1| = 16m/s
$$

$$
p_0 + \frac{1}{2} \rho V_0^2 + \cancel{\rho g h_0} = p_1 + \frac{1}{2} \rho V_1^2 + \cancel{\rho g h_1}
$$

$$
p_0 + \frac{1}{2} \rho V_0^2 = p_1 + \frac{1}{2} \rho V_1^2
$$

$$
p_0 + \frac{1}{2} \rho V_0^2 - \frac{1}{2} \rho V_1^2 = p_1
$$

$$
p_1 = p_0 + \frac{1}{2} \rho (V_0^2 - V_1^2)
$$

$$
p-1 = 200kPa + \frac{1}{2} * 1000kg/m^3 * ((4m/s)^2 - (16m/s)^2) = \boxed{80kPa}
$$
