# AERE 310 HW 4

Abhigyaan Deep

## 1.

$$
\psi(r, \theta) = r^n \sin(\theta)
$$

## 1. (a)

$$
v_r = \frac{1}{r} \frac{\partial \psi}{\partial \theta} = \frac{1}{r} r^n \cos(\theta) = r^{n-1} \cos(\theta)
$$

$$
v_\theta = -\frac{\partial \psi}{\partial r} = -nr^{n-1} \sin(\theta)
$$

$$
\omega = \nabla \times V = \frac{\partial v}{\partial x} - \frac{\partial u}{\partial y} = \frac{1}{r} \frac{\partial}{\partial r} r v_\theta - \frac{1}{r} \frac{\partial v_r}{\partial \theta} = 0
$$

$$
0 = -\frac{1}{r} \frac{\partial}{\partial r} r nr^{n-1} \sin(\theta) - \frac{1}{r} \frac{\partial (r^{n-1} \cos(\theta))}{\partial \theta}
$$

$$
0 = -\frac{1}{r} \frac{\partial}{\partial r} nr^n \sin(\theta) + \frac{1}{r} r^{n-1} \sin(\theta)
$$

$$
0 = -\frac{1}{r} n^2r^{n-1} \sin(\theta) + r^{n-2} \sin(\theta)
$$

$$
0 = -n^2 \cancel{r^{n-2}} \cancel{\sin(\theta)} + \cancel{r^{n-2}} \cancel{\sin(\theta)} = -n^2 + 1
$$

$$
0 = -n^2 + 1
$$

$$
n^2 = 1 \implies \boxed{n = 1}
$$

## 1. (b)

$$
\psi_\text{uniform} = U_\infty r \sin \theta
$$

$$
\psi_\text{doublet} = -\frac{\kappa}{2 \pi r} \sin \theta
$$

$$
\psi = \psi_\text{uniform} + \psi_\text{doublet} = U_\infty r \sin \theta - \frac{\kappa}{2 \pi r} \sin \theta
$$

$$
r = h \implies \psi = 0 = U_\infty h \sin \theta - \frac{\kappa}{2 \pi h} \sin \theta
$$

$$
0 = U_\infty h \cancel{\sin \theta} - \frac{\kappa}{2 \pi h} \cancel{\sin \theta}
$$

$$
0 = U_\infty h - \frac{\kappa}{2 \pi h}
$$

$$
\frac{\kappa}{2 \pi h} = U_\infty h
$$

$$
\kappa = 2 \pi U_\infty h^2
$$

$$
\psi = U_\infty r \sin \theta - \frac{\cancel{2 \pi} U_\infty h^2}{\cancel{2 \pi} r} \sin \theta
$$

$$
\boxed{\psi = U_\infty r \sin \theta - \frac{U_\infty h^2}{r} \sin \theta}
$$

## 2. (a)

Intuitively, $2$ and $3$ should be place perpendicular to $1$, on the top and bottom.

$$
p_2 = p_3 = p_\infty
$$

For a circle (extrapolated to a cylinder) with radius $R$:

$$
\phi_\text{uniform} = V_\infty r \cos \theta
$$

$$
\phi_\text{doublet} = V_\infty \frac{R^2}{r} \cos \theta
$$

$$
\phi = \phi_\text{uniform} + \phi_\text{doublet} = V_\infty r \cos \theta + V_\infty \frac{R^2}{r} \cos \theta = V_\infty \left( r + \frac{R^2}{r} \right) \cos \theta
$$

$$
V_r = \frac{\partial \phi}{\partial r} = V_\infty \left( 1 - \frac{R^2}{r^2} \right) \cos \theta
$$

$$
V_\theta = \frac{1}{r} \frac{\partial \phi}{\partial \theta} = -\frac{1}{r} V_\infty \left( r + \frac{R^2}{r} \right) \sin \theta = -V_\infty \left( 1 + \frac{R^2}{r^2} \right) \sin \theta
$$

$$
r = R \implies V_r = 0
$$

$$
r = R \implies V_\theta = - 2 V_\infty \sin \theta
$$

$$
V = \sqrt{V_r^2 + V_\theta^2} = 2 V_\infty \sin \theta
$$

$$
c_p = 1 - \frac{V^2}{V_\infty^2} = 1 - \frac{4 V_\infty^2 \sin^2 \theta}{V_\infty^2}
$$

$$
p = p_\infty \implies c_p = 0 = 1 - \frac{4 \cancel{V_\infty^2} \sin^2 \theta}{\cancel{V_\infty^2}}
$$

$$
1 = 4 \sin^2 \theta
$$

$$
\pm 1 = 2 \sin \theta
$$

$$
\pm \frac{1}{2} = \sin \theta \implies \theta = \pm 30 \degree, ~ \boxed{\pm 150 \degree}
$$

$\pm30\degree$ with respect to $+x$ isn't quite what I want judging by the fact the holes lie on the left side of the diagram so I am going with $\pm150\degree$.

![](https://i.imgur.com/BbkaTk3m.png)

## 2. (b)

For incompressible, inviscid flow at the stagnation point:

$$
c_p = 1
$$

$$
c_p = \frac{p - p_\infty}{\frac{1}{2} \rho V_\infty^2}
$$

At the stagnation point:

$$
1 = \frac{p_1 - p_\infty}{\frac{1}{2} \rho V_\infty^2}
$$

$$
\frac{1}{2} \rho V_\infty^2 = p_1 - p_\infty
$$

$$
\rho V_\infty^2 = 2p_1 - 2p_\infty
$$

Since $p_2 = p_3 = p_\infty$:

$$
\rho V_\infty^2 = 2p_1 - p_2 - p_3
$$

$$
V_\infty^2 = \frac{2p_1 - p_2 - p_3}{\rho}
$$

$$
\boxed{V_\infty = \sqrt{\frac{2p_1 - p_2 - p_3}{\rho}}}
$$

## 3.

$$
c_\text{p, front} = 1 - 4 \sin^2 \theta
$$

$$
p_\text{back} = p_\infty \implies c_\text{p, back} = \frac{\cancel{p_\infty - p_\infty}}{\frac{1}{2} \rho V_\infty^2} = 0
$$

$$
c_D = \frac{1}{2} \int_0^{2\pi} c_p \cos \theta ~ d\theta = \cancel{\frac{1}{2} \int_{-\frac{\pi}{2}}^{\frac{\pi}{2}} c_\text{p, back} \cos \theta ~ d\theta} + \frac{1}{2} \int_{\frac{\pi}{2}}^{\frac{3\pi}{2}} c_\text{p, front} \cos \theta ~ d\theta
$$

$$
c_D = \frac{1}{2} \int_{\frac{\pi}{2}}^{\frac{3\pi}{2}} (1 - 4 \sin^2 \theta) \cos \theta ~ d\theta
$$

$$
c_D = \frac{1}{2} \int_{\frac{\pi}{2}}^{\frac{3\pi}{2}} \cos \theta - 4 \sin^2 \theta \cos \theta ~ d\theta = \frac{1}{2} \int_{\frac{\pi}{2}}^{\frac{3\pi}{2}} \cos \theta ~ d\theta - \int_{\frac{\pi}{2}}^{\frac{3\pi}{2}} 2 \sin^2 \theta \cos \theta ~ d\theta
$$

$$
c_D = \frac{1}{2} [\sin \theta]_{\frac{\pi}{2}}^{\frac{3\pi}{2}} - \int_{\frac{\pi}{2}}^{\frac{3\pi}{2}} 2 \sin^2 \theta \cos \theta ~ d\theta
$$

$$
c_D = \frac{1}{2} [-2] - \int_{\frac{\pi}{2}}^{\frac{3\pi}{2}} 2 \sin^2 \theta \cos \theta ~ d\theta
$$

$$
c_D = -1 - \int_{\frac{\pi}{2}}^{\frac{3\pi}{2}} 2 \sin^2 \theta \cos \theta ~ d\theta
$$

$$
c_D = -1 - \frac{2}{3} [\sin^3 \theta]_{\frac{\pi}{2}}^{\frac{3\pi}{2}}
$$

$$
c_D = -1 - \frac{2}{3} [-1 - 1]
$$

$$
c_D = -1 + \frac{4}{3}
$$

$$
\boxed{c_D = \frac{1}{3}}
$$

## 4.

$$
M = N + 1
$$

$$
a = 1
$$

$$
\Gamma_0 = 10\pi
$$

$$
P_+ = (1, 10)
$$

$$
P_- = (1, -10)
$$

$$
M = 11 \implies N = 10
$$

$$
M = 101 \implies N = 100
$$

$$
M = 1001 \implies N = 1000
$$

$$
\psi = - \frac{\Gamma}{2\pi} \ln r = - \frac{\Gamma}{2\pi} \ln \sqrt{x^2 + y^2}
$$

The vortices will be offset from the origin:

$$
\psi_n = - \frac{\Gamma_n}{2\pi} \ln \sqrt{(x - x_n)^2 + (y - y_n)^2}
$$

After much experimentation with the equations, I have settled on an iterator $n$ in a summation that goes from $-\frac{N}{2}$ to $\frac{N}{2}$ which gives me $N + 1$ summands instead of going from $0$ to $N$ which introduces a summation inside the $\ln$.

$x$ is a function of $n$ which just paces right with a step size of $a$ as $n$:

$$
x_n = \cancel{a}n = n
$$

All the vortices are on the $y$ axis:

$$
y_n = 0
$$

$\Gamma$ is the same for all:

$$
\Gamma_n = \Gamma_0 = 10 \pi
$$

And, finally the whole summation:

$$
\psi = \sum_{n = -\frac{N}{2}}^{\frac{N}{2}} \psi_n = \sum_{n = -\frac{N}{2}}^{\frac{N}{2}} \ln -\frac{\Gamma_n}{2\pi} \sqrt{(x - x_n)^2 + (y - y_n)^2}
$$

$$
\psi = -\frac{10 \cancel{\pi}}{2 \cancel{\pi}} \sum_{n = -\frac{N}{2}}^{\frac{N}{2}} \ln \sqrt{(x - n)^2 + (y - \cancel{y_n})^2}
$$

$$
\psi = -5 \sum_{n = -\frac{N}{2}}^{\frac{N}{2}} \ln \sqrt{(x - n)^2 + y^2}
$$

$$
\psi = -\frac{5}{2} \sum_{n = -\frac{N}{2}}^{\frac{N}{2}} \ln ((x - n)^2 + y^2)
$$

$$
u = \frac{\partial \psi}{\partial y} = -\frac{5}{2} \sum_{n = -\frac{N}{2}}^{\frac{N}{2}} \frac{2y}{(x - n)^2 + y^2}
$$

$$
v = -\frac{\partial \psi}{\partial x} = -\frac{5}{2} \sum_{n = -\frac{N}{2}}^{\frac{N}{2}} \frac{2(x - n)}{(x - n)^2 + y^2}
$$

$$
u_+ = u(P_+) = -\frac{5}{2} \sum_{n = -\frac{N}{2}}^{\frac{N}{2}} \frac{20}{(1 - n)^2 + 100}
$$

$$
v_+ = v(P_+) = -\frac{5}{2} \sum_{n = -\frac{N}{2}}^{\frac{N}{2}} \frac{2(1 - n)}{(1 - n)^2 + 100}
$$

$$
u_- = u(P_-) = -\frac{5}{2} \sum_{n = -\frac{N}{2}}^{\frac{N}{2}} \frac{-20}{(1 - n)^2 + 100}
$$

$$
v_- = v(P_-) = -\frac{5}{2} \sum_{n = -\frac{N}{2}}^{\frac{N}{2}} \frac{2(1 - n)}{(1 - n)^2 + 100}
$$

$$
V(P) = \langle u(P), v(P) \rangle
$$

$$
N + 1 = 11 \implies V_+ = \langle -4.9988, -0.4206 \rangle
$$

$$
N + 1 = 11 \implies V_- = \langle 4.9988, -0.4206 \rangle
$$

$$
N + 1 = 101 \implies V_+ = \langle -13.7524, -0.1906 \rangle
$$

$$
N + 1 = 101 \implies V_- = \langle 13.7524, -0.1906 \rangle
$$

$$
N + 1 = 1001 \implies V_+ = \langle -15.5082, -0.0200 \rangle
$$

$$
N + 1 = 1001 \implies V_- = \langle 15.5082, -0.0200 \rangle
$$

Wolfram Alpha had a stroke calculating the above so here's the Python code I used where I changed `summand(n)` for every $P$ and between $u$ and $v$ (this is snippet calculates $v$ for $P_-$ which I did last):

```python
def summand(n):
    return (2*(1 - n))/((1 - n)**2 + 100)

def compute_summation(N):
    total = 0
    for n in range(-N // 2, N // 2 + 1):
        total += summand(n)
    return -5 / 2 * total

N = 1000
result = compute_summation(N)
print(result)
```

## 5.

$$
\Lambda = 25 \pi \frac{m^2}{s}
$$

$$
h_1 = 3m
$$

$$
h_2 = 4m
$$

$$
d_1 = 4m
$$

$$
d_2 = 3m
$$

$$
\Lambda_1 = \Lambda_1' = \Lambda
$$

$$
\Lambda_2 = \Lambda_2' = -\Lambda
$$

For the method of images, this is what I came up with where the reflections have the same strengths (which I am indicating with a prime above):

![](https://i.imgur.com/d633jmvl.png)

I am also treating $A = (0, 0)$ as the origin.

$$
P_1 = (-d_1, h_1)
$$

$$
P_1' = (-d_1, -h_1)
$$

$$
P_2 = (d_2, h_2)
$$

$$
P_2' = (d_2, -h_2)
$$

For simplicity (note the $4$ in the denominator instead of $2$, it'll be useful soon):

$$
C \equiv \frac{\Lambda}{4 \pi}
$$

Superpositioning $\psi$ will introduce $\arctan$ when going to rectangular so I rather deal with the $\ln$ in $\phi$:

$$
\phi = \frac{\Lambda}{2 \pi} \ln r = \frac{\Lambda}{2 \pi} \ln r = \frac{\Lambda}{2 \pi} \ln \sqrt{x^2 + y^2} = \frac{\Lambda}{4 \pi} \ln (x^2 + y^2) = C \ln (x^2 + y^2)
$$

$$
\phi_1 = C \ln ((x + d_1)^2 + (y - h_1)^2)
$$

$$
\phi_1' = C \ln ((x + d_1)^2 + (y + h_1)^2)
$$

$$
\phi_2 = -C \ln ((x - d_2)^2 + (y - h_2)^2)
$$

$$
\phi_2' = -C \ln ((x - d_2)^2 + (y + h_2)^2)
$$

$$
\phi = \phi_1 + \phi_1' + \phi_2 + \phi_2'
$$

$$
\frac{\partial \phi}{\partial x} = \frac{\partial \phi_1}{\partial x} + \frac{\partial \phi_1'}{\partial x} + \frac{\partial \phi_2}{\partial x} + \frac{\partial \phi_2'}{\partial x}
$$

$$
u = u_1 + u_1' + u_2 + u_2'
$$

Since it's a wall at $A = (0, 0)$, $v$ has to be $0$, saving me some work:

$$
v = 0
$$

All hell breaks loose for $u$:

$$
u_1 = \frac{\partial \phi_1}{\partial x} = \frac{2 C (x + d_1)}{(x + d_1)^2 + (y - h_1)^2}
$$

$$
u_1' = \frac{\partial \phi_1'}{\partial x} = \frac{2 C (x + d_1)}{(x + d_1)^2 + (y + h_1)^2}
$$

$$
u_2 = \frac{\partial \phi_2}{\partial x} = \frac{-2 C (x - d_2)}{(x - d_2)^2 + (y - h_2)^2}
$$

$$
u_2' = \frac{\partial \phi_2'}{\partial x} = \frac{-2 C (x - d_2)}{(x - d_2)^2 + (y + h_2)^2}
$$

$$
u_1(A) = \frac{2 C d_1}{d_1^2 + h_1^2}
$$

$$
u_1'(A) = \frac{2 C d_1}{d_1^2 + h_1^2}
$$

$$
u_2(A) = \frac{2 C d_2}{d_2^2 + h_2^2}
$$

$$
u_2'(A) = \frac{2 C d_2}{d_2^2 + h_2^2}
$$

$$
u(A) = 2u_1(A) + 2u_2(A)
$$

$$
u(A) = \frac{4 C d_1}{d_1^2 + h_1^2} + \frac{4 C d_2}{d_2^2 + h_2^2}
$$

$$
u(A) = 4C \left[ \frac{d_1}{d_1^2 + h_1^2} + \frac{d_2}{d_2^2 + h_2^2} \right] = \frac{\Lambda}{\pi} \left[ \frac{d_1}{d_1^2 + h_1^2} + \frac{d_2}{d_2^2 + h_2^2} \right]
$$

$$
u(A) = \frac{25 \pi \frac{m^2}{s}}{\pi} \left[ \frac{4m}{(4m)^2 + (3m)^2} + \frac{3m}{(3m)^2 + (4m)^2} \right] = \boxed{7m/s}
$$
