# AERE 310 HW 5

Abhigyaan Deep

## 1.

$$
y_u = 16 \frac{x}{c} (1 - \frac{x}{c}) ~ \text{mm}
$$

$$
y_l = 8 \frac{x}{c} (1 - \frac{x}{c}) ~ \text{mm}
$$

$$
c = 4 ~ \text{cm} = 40 ~ \text{mm}
$$

The average of both surfaces should be the camber line:

$$
\eta_c = \frac{y_u + y_l}{2} = \frac{1}{2} \left [ 16 \frac{x}{c} (1 - \frac{x}{c}) + 8 \frac{x}{c} (1 - \frac{x}{c}) \right] = 12 \frac{x}{c} (1 - \frac{x}{c})
$$

For ease of differentiation, I am declaring:

$$
x' = \frac{x}{c}
$$

$$
\frac{d x'}{dx} = \frac{1}{c}
$$

$$
\eta_c = 12 x' (1 - x')
$$

$$
\frac{d \eta_c}{dx'} = 12 (1 - x') + 12x'(-1) = 12 - 12x' - 12x' = 12 - 24x'
$$

$$
\frac{d \eta_c}{dx} = \frac{d \eta_c}{dx'} \frac{d x'}{dx} = (12 - 24x') \frac{1}{c} = (12 - 24 \frac{x}{c}) \frac{1}{c} = \frac{12}{c} - \frac{24}{c^2} x
$$

$$
x = \frac{c}{2} (1 - \cos \theta)
$$

$$
\frac{d \eta_c}{dx} = \frac{12}{c} - \frac{24}{c^2} \frac{c}{2} (1 - \cos \theta) = \frac{12}{c} - \frac{12}{c} (1 - \cos \theta)
$$

$$
\frac{d \eta_c}{dx} = \frac{12}{c} (1 - 1 + \cos \theta) = \frac{12}{c} \cos \theta
$$

$$
\frac{d \eta_c}{dx} = A_0 + A_1 \cos \theta + A_2 \cos 2 \theta
$$

$$
\implies A_0 = 0, ~ A_1 = \frac{12}{c}, ~ A_2 = 0
$$

$$
\alpha_{L=0} = \cancel{A_0} - \frac{A_1}{2} = \frac{1}{2} \frac{12}{c} = \frac{6}{c}
$$

$$
c_l = 2 \pi (\alpha - \alpha_{L=0}) = 2 \pi (\alpha - \frac{6}{c}) = 2 \pi (\alpha - \frac{6}{40}) = \boxed{2 \pi (\alpha - \frac{3}{20})}
$$

$$
c_{m_{c/4}} = \frac{\pi}{4} (\cancel{A_2} - A_1) = -\frac{\pi}{4} A_1 = -\frac{\pi}{4} \frac{12}{c} = -\frac{\pi}{4} \frac{12}{40} = \boxed{-\frac{3 \pi}{40}}
$$

## 2.

$$
\alpha_{L=0} = -3\degree = -0.05236
$$

$$
a = \frac{0.1}{1\degree} = 5.730
$$

$$
c_L = a (\alpha - \alpha_{L=0})
$$

## 2. (a)

$$
\alpha = 5\degree = 0.08727
$$

$$
c_L = 5.730 * (0.08727 - (-0.05236)) = \boxed{0.8001}
$$

## 2. (b)

The slope's the same but now the intercept is opposite:

$$
\alpha_{L=0} = 3\degree = 0.05236
$$

$$
\alpha = -5\degree = -0.08727
$$

$$
c_L = 5.730 * (-0.08727 - 0.05236) = \boxed{-0.8001}
$$

## 2. (c)

Still, the intercept is different here.

$$
c_L(5\degree) = 0.8001 = a (\alpha - \alpha_{L=0})
$$

$$
\alpha = \frac{c_L(5\degree)}{a} + \alpha_{L=0} = \frac{0.8001}{5.730} + 0.05236 = 0.1920 = \boxed{11.00\degree}
$$

## 3.

$$
\frac{\eta_c}{c} =
\begin{cases}
  0.25 \left[ 0.8 \frac{x}{c} - (\frac{x}{c})^2 \right] & \text{for } 0 \leq \frac{x}{c} \leq 0.4 \\
  0.111 \left[ 0.2 + 0.8 \frac{x}{c} - (\frac{x}{c})^2 \right] & \text{for } 0.4 \leq \frac{x}{c} \leq 1
\end{cases}
$$

## 3. (a)

$$
\alpha_{L=0} = 3\degree = 0.05236
$$

$$
\eta_c =
\begin{cases}
  0.25 \left[ 0.8 x - \frac{1}{c}x^2 \right] & \text{for } 0 \leq x \leq 0.4c \\
  0.111 \left[ 0.2c + 0.8x - \frac{1}{c}x^2 \right] & \text{for } 0.4c \leq x \leq c
\end{cases}
$$

$$
\frac{d \eta_c}{dx} =
\begin{cases}
  0.25 \left[ 0.8 - \frac{2}{c}x \right] & \text{for } 0 \leq x \leq 0.4c \\
  0.111 \left[ 0.8 - \frac{2}{c}x \right] & \text{for } 0.4c \leq x \leq c
\end{cases}
$$

$$
\frac{d \eta_c}{dx} =
\begin{cases}
  0.2 - \frac{0.5}{c}x & \text{for } 0 \leq x \leq 0.4c \\
  0.0888 - \frac{0.222}{c}x & \text{for } 0.4c \leq x \leq c
\end{cases}
$$

The first bound:

$$
x = \frac{c}{2} (1 - \cos \theta)
$$

$$
x = 0 \implies 0 = \frac{c}{2} (1 - \cos \theta)
$$

$$
0 = 1 - \cos \theta
$$

$$
\cos \theta = 1 \implies \theta = 0
$$

The second bound:

$$
x = 0.4c \implies 0.4\cancel{c} = \frac{\cancel{c}}{2} (1 - \cos \theta)
$$

$$
0.8 = 1 - \cos \theta \implies \theta = 1.369
$$

The third bound:

$$
x = c \implies \cancel{c} = \frac{\cancel{c}}{2} (1 - \cos \theta)
$$

$$
2 = 1 - \cos \theta \implies \theta = \pi
$$

$$
\frac{d \eta_c}{dx} =
\begin{cases}
  0.2 - \frac{0.5}{c} \frac{c}{2} (1 - \cos \theta) & \text{for } 0 \leq \theta \leq 1.369 \\
  0.0888 - \frac{0.222}{c} \frac{c}{2} (1 - \cos \theta) & \text{for } 1.369 \leq x \leq \pi
\end{cases}
$$

$$
\frac{d \eta_c}{dx} =
\begin{cases}
  0.25 \cos \theta - 0.05 & \text{for } 0 \leq \theta \leq 1.369 \\
  0.111 \cos \theta - 0.0222 & \text{for } 1.369 \leq x \leq \pi
\end{cases}
$$

To reduce the syntax insanity, I am declaring:

$$
\frac{d \eta_c}{dx} =
\begin{cases}
  H_A & \text{for } 0 \leq \theta \leq 1.369 \\
  H_B & \text{for } 1.369 \leq x \leq \pi
\end{cases}
$$

Where:

$$
H_A = 0.25 \cos \theta - 0.05
$$

$$
H_B = 0.111 \cos \theta - 0.0222
$$

Thus:

$$
A_0 = \frac{1}{\pi} \int_0^\pi \frac{d \eta_c}{dx} d\theta = \frac{1}{\pi} \left [ \int_0^{1.369} H_A ~ d\theta + \int_{1.369}^\pi H_B ~ d\theta \right]
$$

$$
\int_0^{1.369} H_A ~ d\theta = \int_0^{1.369} 0.25 \cos \theta - 0.05 ~ d\theta = 0.1765
$$

$$
\int_{1.369}^\pi H_B ~ d\theta = \int_{1.369}^\pi 0.111 \cos \theta - 0.0222 ~ d\theta = -0.1481
$$

$$
A_0 = \frac{1}{\pi} [ 0.1765 - 0.1481] = 9.040 \times 10^{-3}
$$

Moreover:

$$
A_1 = \frac{2}{\pi} \int_0^\pi \frac{d \eta_c}{dx} \cos \theta ~ d\theta = \frac{2}{\pi} \left[ \int_0^{1.369} H_A \cos \theta ~ d\theta + \int_{1.369}^\pi H_B \cos \theta ~ d\theta \right]
$$

$$
\int_0^{1.369} H_A \cos \theta ~ d\theta = \int_0^{1.369} (0.111 \cos \theta - 0.0222) \cos \theta ~ d\theta = 0.06513
$$

$$
\int_{1.369}^\pi H_B \cos \theta ~ d\theta = \int_{1.369}^\pi (0.111 \cos \theta - 0.0222) \cos \theta ~ d\theta = 0.1092
$$

$$
A_1 = \frac{2}{\pi} \left[ 0.06513 + 0.1092 \right] = 0.1110
$$

Finally:

$$
\alpha_{L=0} = A_0 - \frac{A_1}{2} = 9.040 \times 10^{-3} - \frac{0.1110}{2} = -0.04646
$$

$$
c_l = 2\pi (\alpha - \alpha_{L=0}) = 2\pi (0.05236 - (-0.04646)) = \boxed{0.6209}
$$

## 3. (b)

$$
\alpha_{L=0} = 3\degree = 0.05236
$$

$$
A_2 = \frac{2}{\pi} \int_0^\pi \frac{d \eta_c}{dx} \cos 2\theta ~ d\theta = \frac{2}{\pi} \left[ \int_0^{1.369} H_A \cos 2\theta ~ d\theta + \int_{1.369}^\pi H_B \cos 2\theta ~ d\theta \right]
$$

$$
\int_0^{1.369} H_A \cos 2\theta ~ d\theta = \int_0^{1.369} (0.25 \cos \theta - 0.05) \cos 2\theta ~ d\theta = 0.0784
$$

$$
\int_{1.369}^\pi H_B \cos 2\theta ~ d\theta = \int_{1.369}^\pi (0.111 \cos \theta - 0.0222) \cos 2\theta ~ d\theta = -0.03480
$$

$$
A_2 = \frac{2}{\pi} \left[ 0.0784 - 0.03480 \right] = 0.02776
$$

$$
c_{m_{c/4}} = \frac{\pi}{4} (A_2 - A_1) = \frac{\pi}{4} (0.02776 - 0.1110) = \boxed{-0.06538}
$$

$$
x_{cp} = \frac{c}{4} \left[ 1 + \frac{\pi (A_1 - A_2)}{c_l} \right]
$$

$$
x_{cp}/c = \frac{1}{4} \left[ 1 + \frac{\pi (A_1 - A_2)}{c_l} \right]
$$

$$
x_{cp}/c = \frac{1}{4} \left[ 1 + \frac{\pi (0.1110 - 0.02776)}{0.6209} \right] = \boxed{0.3553}
$$

## 3. (c)

![](https://i.imgur.com/qndZTUk.png)

Pretty darn close.

## 3. (d)

$$
h = 3km
$$

$$
V_\infty = 60m/s
$$

$$
c = 2m
$$

$$
\rho = 9.0925 \times 10^{-1} \frac{kg}{m^3}
$$

$$
q = \frac{1}{2} \rho V_\infty^2 = \frac{1}{2} * 9.0925 \times 10^{-1} \frac{kg}{m^3} * (60m/s)^2 = 1.637kPa
$$

$$
L' = c_l q c = 0.6209 * 1.637kPa * 2m = \boxed{2.033 kN/m}
$$

## 4.

The piecewise function:

$$
\eta_c =
\begin{cases}
  \eta_A & \text{for } 0 \leq x \leq 0.1c \\
  \eta_B & \text{for } 0.1c \leq x \leq 0.7c \\
  \eta_C & \text{for } 0.7c \leq x \leq c \\
\end{cases}
$$

The pieces:

$$
\eta_A = \frac{0.02c}{0.1c}x - 0.02c = 0.2x - 0.02c
$$

$$
\eta_B = 0
$$

$$
\eta_C = \frac{-0.05c}{0.3c}(x - 0.7c) = 0.1167 c - 0.1667 x
$$

Derivatives:

$$
H_A = \frac{d \eta_a}{dx} = 0.2
$$

$$
H_B = \frac{d \eta_b}{dx} = 0
$$

$$
H_C = \frac{d \eta_c}{dx} = -0.1667
$$

Bounds in polar:

$$
x = 0 \implies \theta = 0
$$

$$
x = 0.1c = \frac{c}{2} (1 - \cos \theta) \implies x = 0.6435
$$

$$
x = 0.7c = \frac{c}{2} (1 - \cos \theta) \implies x = 1.982
$$

$$
x = c \implies \theta = \pi
$$

$$
\frac{d\eta_c}{dx} =
\begin{cases}
  0.2 & \text{for } 0 \leq \theta \leq 0.6435 \\
  0 & \text{for } 0.6435 \leq \theta \leq 1.982 \\
  -0.1667 & \text{for } 1.982 \leq \theta \leq \pi \\
\end{cases}
$$

## 4. (a)

$$
A_0 = \frac{1}{\pi} \int_0^\pi \frac{d \eta_c}{dx} d\theta = \frac{1}{\pi} \left[ 0.2(0.6435 - 0) + 0(1.982 - 0.6435) - 0.1667(\pi - 1.982) \right] = -0.02056
$$

$$
A_1 = \frac{2}{\pi} \int_0^\pi \frac{d \eta_c}{dx} \cos \theta ~ d\theta = \frac{2}{\pi} \left[ \int_0^{0.6435} 0.2 \cos \theta ~ d\theta + \cancel{\int_{0.6435}^{1.982} 0 \cos \theta ~ d\theta} - \int_{1.982}^\pi 0.1667 \cos \theta ~ d\theta \right]
$$

$$
A_1 = \frac{2}{\pi}[0.12 - (-0.152804)] = 0.1737
$$

$$
\alpha_{L=0} = A_0 - \frac{A_1}{2} = -0.02056 - \frac{0.1737}{2} = -0.1074 = \boxed{-6.154\degree}
$$

## 4. (b)

$$
\rho = \rho_\infty = 1.2\frac{kg}{m^3}
$$

$$
V_\infty = 50m/s
$$

$$
\alpha = 2\degree = 0.03491
$$

$$
c = 2m
$$

$$
c_l = 2\pi (\alpha - \alpha_{L=0}) = 2\pi (0.03491 - (-0.1074)) = 0.8942
$$

$$
q = \frac{1}{2} \rho V_\infty^2 = \frac{1}{2} * 1.2\frac{kg}{m^3} * (50m/s)^2 = 1.5kPa
$$

$$
L' = c_l q c = 0.8942 * 1.5kPa * 2m = \boxed{2.683kN/m}
$$

$$
A_2 = \frac{2}{\pi} \int_0^\pi \frac{d \eta_c}{dx} \cos 2\theta ~ d\theta = \frac{2}{\pi} \left[ \int_0^{0.6435} 0.2 \cos 2\theta ~ d\theta + \cancel{\int_{0.6435}^{1.982} 0 \cos 2\theta ~ d\theta} - \int_{1.982}^\pi 0.1667 \cos 2\theta ~ d\theta \right]
$$

$$
A_2 = \frac{2}{\pi} \left[ 0.09600 - 0.06108 \right] = 0.02223
$$

$$
c_{m_{c/4}} = \frac{\pi}{4} (A_2 - A_1) = \frac{\pi}{4} (0.02223 - 0.1737) = -0.1190
$$

$$
c_{m_{LE}} = c_{m_{c/4}} - \frac{1}{4}c_l = -0.1190 - \frac{1}{4} * 0.8942 = -0.3426
$$

$$
M_{LE}' = q c^2 c_{m_{LE}} = 1.5kPa * (2m)^2 * -0.3426 = \boxed{-2.06kN}
$$
